soundness of unification with structural polymorphism

ML_SP_Unify.v
@@ -15,29 +15,82 @@ Module Infra := MkInfra(Cstr)(Const).
 Import Infra.
 Import Defs.
 
-Definition add_binding x (T:typ) S := map (typ_subst (x ~ T)) S & x ~ T.
+Definition compose S1 S2 := map (typ_subst S1) S2 & S1.
 
-Fixpoint unify (pairs:list (typ*typ)) (S:Env.env typ) (h:nat) {struct h}
-  : option (Env.env typ) :=
+Parameter unique : Cstr.cstr -> list var.
+Parameter unique_ok : forall c l, In l (unique c) <-> Cstr.unique c l.
+Parameter cstr_lub : Cstr.cstr -> Cstr.cstr -> Cstr.cstr.
+Parameter cstr_lub_ok : forall c1 c2 c,
+  (Cstr.entails c c1 /\ Cstr.entails c c2) <-> Cstr.entails c (cstr_lub c1 c2).
+
+Fixpoint unify_kind_rel (kr kr':list(var*typ)) (un:list var)
+  (pairs:list(typ*typ)) {struct kr} :=
+  match kr with
+  | nil => (kr', pairs)
+  | (l,T)::krem =>
+    if In_dec eq_var_dec l un then
+      match get l kr' with
+      | None => unify_kind_rel krem ((l,T)::kr') un pairs
+      | Some T' => unify_kind_rel krem kr' un ((T,T')::pairs)
+      end
+    else unify_kind_rel krem ((l,T)::kr') un pairs
+  end.
+
+Fixpoint remove_env (A:Set) (E:Env.env A) (x:var) {struct E} : Env.env A :=
+  match E with
+  | nil => nil
+  | (y,a)::E' =>
+    if x == y then E' else (y,a) :: remove_env E' x
+  end.
+
+Definition unify_kinds (k1 k2:kind) :=
+  match k1, k2 with
+  | None, _ => (k2, nil)
+  | Some _, None => (k1, nil)
+  | Some (Kind kc1 kr1), Some (Kind kc2 kr2) =>
+    let kc := cstr_lub kc1 kc2 in
+    let (kr, pairs) := unify_kind_rel (kr1 ++ kr2) nil (unique kc) nil in
+    (Some (Kind kc kr), pairs)
+  end.
+
+Definition unify_vars (K:kenv) (x y:var) :=
+  match get x K, get y K with
+  | Some k1, Some k2 =>
+    let (k, pairs) := unify_kinds k1 k2 in
+    Some (remove_env (remove_env K x) y & y ~ k, pairs)
+  | _, _ => None
+  end.
+
+Definition unify_nv (unify : kenv -> subs -> option (kenv * subs)) K S x T :=
+  if S.mem x (typ_fv T) then None else
+    match get x K with
+    | Some None => unify (remove_env K x) (compose (x ~ T) S)
+    | _ => None
+    end.
+
+Fixpoint unify (h:nat) (pairs:list (typ*typ)) (K:kenv) (S:subs) {struct h}
+  : option (kenv * subs) :=
   match h with 0 => None
   | S h' =>
     match pairs with
-    | nil => Some S
+    | nil => Some (K,S)
     | (T1,T2) :: pairs' =>
       match typ_subst S T1, typ_subst S T2 with
       | typ_bvar n, typ_bvar m =>
-        if n === m then unify pairs' S h' else None
+        if n === m then unify h' pairs' K S else None
       | typ_fvar x, typ_fvar y =>
-        if x == y then unify pairs' S h' else
-        unify pairs' (add_binding x (typ_fvar y) S) h'
+        if x == y then unify h' pairs' K S else
+        match unify_vars (map (kind_subst S) K) x y with
+        | Some (K', pairs) =>
+          unify h' (pairs ++ pairs') K' (compose (x ~ typ_fvar y) S)
+        | None => None
+        end
       | typ_fvar x, T =>
-        if S.mem x (typ_fv T) then None else
-        unify pairs' (add_binding x T S) h'
+        unify_nv (unify h' pairs') K S x T 
       | T, typ_fvar x =>
-        if S.mem x (typ_fv T) then None else
-        unify pairs' (add_binding x T S) h'
-      | typ_arrow T11 T12, typ_arrow T21 T22 =>
-        unify ((T11,T21)::(T12,T22)::pairs') S h'
+        unify_nv (unify h' pairs') K S x T 
+       | typ_arrow T11 T12, typ_arrow T21 T22 =>
+        unify h' ((T11,T21)::(T12,T22)::pairs') K S
       | _, _ =>
         None
       end
@@ -73,6 +126,32 @@ Proof.
   apply* IHS.
 Qed.
 
+Lemma typ_subst_compose : forall S1 S2 T,
+  disjoint (dom S1) (dom S2) ->
+  typ_subst (compose S1 S2) T =
+  typ_subst S1 (typ_subst S2 T).
+Proof.
+  induction T; simpl; intros; auto.
+    unfold compose.
+    simpl; case_eq (get v S1); intros.
+      rewrite* (binds_prepend (map (typ_subst S1) S2) H0).
+      case_eq (get v S2); intros.
+        destruct (H v). elim (binds_fresh H0 H2).
+        elim (binds_fresh H1 H2).
+      simpl; rewrite* H0.
+    case_eq (get v S2); intros.
+      rewrite* (binds_concat_fresh S1 (binds_map (typ_subst S1) H1)).
+      destruct* (H v). elim (binds_fresh H1 H2).
+    simpl; rewrite H0.
+    case_eq (get v (map (typ_subst S1) S2 & S1)); intros; auto.
+    destruct (binds_concat_inv H2).
+      destruct H3. destruct (binds_map_inv _ _ H4).
+      destruct H5; rewrite H6 in H1; discriminate.
+    rewrite H3 in H0; discriminate.
+  rewrite* IHT1.
+  rewrite* IHT2.
+Qed.
+
 Lemma binds_typ_subst : forall x T S,
   binds x T S -> typ_subst S (typ_fvar x) = T.
 Proof.
@@ -106,10 +185,10 @@ Qed.
 Lemma add_binding_is_subst : forall S x T,
   is_subst S ->
   disjoint (dom S \u {{x}}) (typ_fv T) ->
-  is_subst (add_binding x T S).
+  is_subst (compose (x ~ T) S).
 Proof.
   intros.
-  unfold add_binding.
+  unfold compose.
   intro; intros.
   binds_cases H1.
     destruct (binds_map_inv _ _ B) as [b [F B']].
@@ -123,36 +202,6 @@ Qed.
 
 Ltac case_rewrite t H :=
   case_eq t; introv H; rewrite H in *; try discriminate.
-
-Lemma map_get_None : forall (A:Set) (f:A->A) v S,
-  get v S = None -> get v (map f S) = None.
-Proof.
-  induction S; simpl; intros. auto.
-  destruct a.
-  simpl.
-  destruct (v == v0). discriminate. auto.
-Qed.
-
-Lemma typ_subst_add_binding : forall x T' S T,
-  x \notin dom S ->
-  typ_subst (add_binding x T' S) T =
-  typ_subst (x ~ T') (typ_subst S T).
-Proof.
-  induction T; simpl; intros; auto.
-    destruct (v == x).
-      subst.
-      case_eq (get x S); intros.
-        elim (binds_fresh H0 H).
-      simpl. destruct* (x == x).
-    case_eq (get v S); intros.
-      use (binds_map (typ_subst (x ~ T')) H0).
-      unfold binds in H1; rewrite* H1.
-    rewrite (map_get_None (typ_subst (x ~ T')) _ _ H0).
-    simpl.
-    destruct* (v == x).
-  rewrite* IHT1.
-  rewrite* IHT2.
-Qed.
 
 Lemma typ_subst_disjoint : forall S T,
   is_subst S -> disjoint (dom S) (typ_fv (typ_subst S T)).
@@ -170,53 +219,81 @@ Lemma binds_add_binding : forall S T0 T1 v x T,
   is_subst S ->
   typ_subst S T0 = typ_fvar v ->
   binds x (typ_subst S T) S ->
-  binds x (typ_subst (add_binding v T1 S) T) (add_binding v T1 S).
+  binds x (typ_subst (compose (v ~ T1) S) T) (compose (v ~ T1) S).
 Proof.
   intros.
   use (typ_subst_disjoint T0 H).
     rewrite H0 in H2. simpl in H2.
-  rewrite* typ_subst_add_binding.
-  unfold add_binding.
-  apply binds_concat_fresh.
-    apply* binds_map.
-  destruct* (H2 x).
-  elim (binds_fresh H1 H3).
+  rewrite typ_subst_compose.
+    unfold compose.
+    apply binds_concat_fresh.
+      apply* binds_map.
+    simpl. rewrite union_empty_r; intro.
+    rewrite (S.singleton_1 H3) in H2.
+    destruct* (H2 x).
+    elim (binds_fresh H1 H4).
+  simpl; disjoint_solve.
 Qed.
 
-Lemma unify_keep : forall h pairs S0 S,
-  unify pairs S0 h = Some S ->
-  is_subst S0 ->
-  is_subst S /\
-  forall x T, binds x (typ_subst S0 T) S0 -> binds x (typ_subst S T) S.
+Lemma unify_keep_nv : forall h pairs K K' T S S' t t0 v,
+  (forall K S,
+    unify h pairs K S = Some (K', S') ->
+    is_subst S ->
+    is_subst S' /\
+    (forall (x : var) (T : typ),
+      binds x (typ_subst S T) S -> binds x (typ_subst S' T) S')) ->
+  is_subst S ->
+  typ_subst S t = typ_fvar v ->
+  typ_subst S t0 = T ->
+  unify_nv (unify h pairs) K S v T = Some (K', S') ->
+  is_subst S' /\
+  (forall (x : var) (T : typ),
+    binds x (typ_subst S T) S -> binds x (typ_subst S' T) S').
+Proof.
+  intros until v. intros IHh HS R1 R2 H.
+  unfold unify_nv in H; simpl in H.
+  case_rewrite (S.mem v (typ_fv T)) R3.
+  fold kind in *.
+  destruct (get v K); try discriminate.
+  destruct k. discriminate.
+  destruct (IHh _ _ H); clear IHh.
+    apply* add_binding_is_subst.
+    simpl.
+    use (typ_subst_disjoint t0 HS). rewrite R2 in H0.
+    disjoint_solve.
+    destruct* (v0 == v). subst*.
+  split*.
+  intros; apply H1.
+  apply* binds_add_binding.
+Qed.
+
+Lemma unify_keep : forall h pairs K S K' S',
+  unify h pairs K S = Some (K', S') ->
+  is_subst S ->
+  is_subst S' /\
+  forall x T, binds x (typ_subst S T) S -> binds x (typ_subst S' T) S'.
 Proof.
   induction h; simpl; intros. discriminate.
   destruct pairs.
     inversions H.
     auto.
   destruct p.
-  case_rewrite (typ_subst S0 t) R1; case_rewrite (typ_subst S0 t0) R2.
+  case_rewrite (typ_subst S t) R1; case_rewrite (typ_subst S t0) R2.
         destruct (n === n0).
-          apply* (IHh _ _ _ H).
+          apply* (IHh _ _ _ _ _ H).
         discriminate.
-       simpl in H.
-       case_rewrite (S.mem v {}) R3.
-       destruct (IHh _ _ _ H); clear IHh.
-         apply* add_binding_is_subst.
-         simpl. intro; auto.
-       split*.
-       intros; apply H2; clear H2.
-       apply* binds_add_binding.
-      simpl in H.
-      destruct (S.mem v {}); try discriminate.
-      destruct (IHh _ _ _ H); clear IHh.
-        apply* add_binding_is_subst.
-        simpl. intro; auto.
-      split*.
-      intros; apply H2.
-      apply* binds_add_binding.
+       apply* (@unify_keep_nv h pairs K K' (typ_bvar n)).
+       intros. apply* IHh.
+      apply* (@unify_keep_nv h pairs K K' (typ_bvar n)).
+      intros. apply* IHh.
      destruct (v == v0).
-       destruct* (IHh _ _ _ H).
-     destruct (IHh _ _ _ H); clear IHh.
+       destruct* (IHh _ _ _ _ _ H).
+     unfold unify_vars in H.
+     remember (map (kind_subst S) K) as K0.
+     destruct (get v K0); try discriminate.
+     destruct (get v0 K0); try discriminate.
+     destruct (unify_kinds k k0).
+     destruct (IHh _ _ _ _ _ H); clear IHh.
        apply* add_binding_is_subst.
        simpl.
        use (typ_subst_disjoint t0 H0). rewrite R2 in H1. simpl in H1.
@@ -225,25 +302,11 @@ Proof.
      split*.
      intros; apply H2.
      apply* binds_add_binding.
-    case_rewrite (S.mem v (typ_fv (typ_arrow t1 t2))) R3.
-    destruct (IHh _ _ _ H); clear IHh.
-      apply* add_binding_is_subst.
-      use (typ_subst_disjoint t0 H0). rewrite R2 in H1.
-      use (notin_disjoint (mem_3 R3)).
-      disjoint_solve.
-    split*.
-    intros; apply H2; clear H2.
-    apply* binds_add_binding.
-   case_rewrite (S.mem v (typ_fv (typ_arrow t1 t2))) R3.
-   destruct (IHh _ _ _ H); clear IHh.
-     apply* add_binding_is_subst.
-     use (typ_subst_disjoint t H0). rewrite R1 in H1.
-     use (notin_disjoint (mem_3 R3)).
-     disjoint_solve.
-    split*.
-    intros; apply H2; clear H2.
-    apply* binds_add_binding.
-  destruct* (IHh _ _ _ H); clear IHh.
+    apply* (@unify_keep_nv h pairs K K' (typ_arrow t1 t2)).
+    intros. apply* IHh.
+   apply* (@unify_keep_nv h pairs K K' (typ_arrow t1 t2)).
+   intros. apply* IHh.
+  destruct* (IHh _ _ _ _ _ H); clear IHh.
 Qed.
 
 Lemma typ_subst_idem : forall S T,
@@ -269,20 +332,20 @@ Proof.
   congruence.
 Qed.
 
-Lemma typ_subst_extend : forall pairs S0 h S T,
-  is_subst S0 ->
-  unify pairs S0 h = Some S ->
-  typ_subst S (typ_subst S0 T) = typ_subst S T.
+Lemma typ_subst_extend : forall h pairs K S K' S' T,
+  is_subst S ->
+  unify h pairs K S = Some (K', S') ->
+  typ_subst S' (typ_subst S T) = typ_subst S' T.
 Proof.
   intros.
-  destruct* (unify_keep _ _ H0).
+  destruct* (unify_keep _ _ _ H0).
   clear H0.
   induction T; intros. simpl*.
-    remember (typ_subst S0 (typ_fvar v)) as T'.
-    use (f_equal (typ_subst S0) HeqT').
+    remember (typ_subst S (typ_fvar v)) as T'.
+    use (f_equal (typ_subst S) HeqT').
     rewrite typ_subst_idem in H0; auto.
     simpl in H0.
-    case_rewrite (get v S0) R.
+    case_rewrite (get v S) R.
       subst.
       use (H2 _ _ R).
       rewrite* (binds_typ_subst H0).
@@ -290,35 +353,47 @@ Proof.
   simpl. congruence.
 Qed.
 
-Lemma unify_var : forall S0 T1 T2 v T pairs h pairs' h' S,
-  typ_subst S0 T1 = typ_fvar v ->
-  typ_subst S0 T2 = T ->
-  unify pairs' S0 h' = Some S ->
-  unify pairs (add_binding v T S0) h = Some S ->
-  is_subst S0 ->
-  v \notin typ_fv T ->
-  typ_subst S T1 = typ_subst S T2.
+Lemma unify_types_nv : forall S T1 T2 v T h' pairs' h pairs K K' S',
+  typ_subst S T1 = typ_fvar v ->
+  typ_subst S T2 = T ->
+  unify h' pairs' K S = Some (K', S') ->
+  unify_nv (unify h pairs) K S v T = Some (K', S') ->
+  is_subst S ->
+  typ_subst S' T1 = typ_subst S' T2.
 Proof.
   intros.
-  assert (is_subst (add_binding v T S0)).
+  unfold unify_nv in H2.
+  case_rewrite (S.mem v (typ_fv T)) R.
+  assert (is_subst (compose (v ~ T) S)).
     apply* add_binding_is_subst.
     use (typ_subst_disjoint T2 H3).
-    rewrite H0 in H5.
-    use (notin_disjoint H4).
+    rewrite H0 in H4.
+    use (notin_disjoint (mem_3 R)).
     disjoint_solve.
-  rewrite <- (typ_subst_extend _ _ T1 H3 H1).
+  rewrite <- (typ_subst_extend _ _ _ T1 H3 H1).
   rewrite H.
-  rewrite <- (typ_subst_extend _ _ (typ_fvar v) H5 H2).
-  rewrite <- (typ_subst_extend _ _ T2 H3 H1).
-  apply (f_equal (typ_subst S)).
+  fold kind in *.
+  case_rewrite (get v K) R1. destruct k. discriminate.
+  rewrite <- (typ_subst_extend _ _ _ (typ_fvar v) H4 H2).
+  rewrite <- (typ_subst_extend _ _ _ T2 H3 H1).
+  apply (f_equal (typ_subst S')).
   simpl. destruct* (v==v).
 Qed.
 
-Theorem unify_sound : forall h pairs S0 S,
-  unify pairs S0 h = Some S ->
-  is_subst S0 ->
+Lemma typ_subst_res_fresh : forall S T v,
+  is_subst S -> typ_subst S T = typ_fvar v -> v # S.
+Proof.
+  intros.
+  use (typ_subst_disjoint T H).
+  rewrite H0 in H1.
+  simpl in H1. destruct* (H1 v).
+Qed.
+
+Theorem unify_types : forall h pairs K S K' S',
+  unify h pairs K S = Some (K',S') ->
+  is_subst S ->
   forall T1 T2,
-    In (T1,T2) pairs -> typ_subst S T1 = typ_subst S T2.
+    In (T1,T2) pairs -> typ_subst S' T1 = typ_subst S' T2.
 Proof.
   induction h; intros. discriminate.
   poses H' H.
@@ -327,54 +402,76 @@ Proof.
     elim H1.
   simpl in H1; destruct H1.
     subst.
-    case_rewrite (typ_subst S0 T1) R1; case_rewrite (typ_subst S0 T2) R2;
+    case_rewrite (typ_subst S T1) R1; case_rewrite (typ_subst S T2) R2;
       try case_rewrite (S.mem v (typ_fv (typ_bvar n))) R3;
       try case_rewrite (S.mem v (typ_fv (typ_arrow t t0))) R3.
           destruct (n === n0).
             subst.
-            rewrite <- (typ_subst_extend _ _ T1 H0 H').
-            rewrite <- (typ_subst_extend _ _ T2 H0 H').
+            rewrite <- (typ_subst_extend _ _ _ T1 H0 H').
+            rewrite <- (typ_subst_extend _ _ _ T2 H0 H').
             congruence.
           discriminate.
          symmetry.
-         apply* (unify_var _ _ _ _ _ _ R2 R1 H' H).
-        apply* (unify_var _ _ _ _ _ _ R1 R2 H' H).
+         apply* (unify_types_nv _ _ _ _ _ _ _ R2 R1 H' H).
+        apply* (unify_types_nv _ _ _ _ _ _ _ R1 R2 H' H).
        destruct (v == v0).
          subst.
-         rewrite <- (typ_subst_extend _ _ T1 H0 H').
-         rewrite <- (typ_subst_extend _ _ T2 H0 H').
+         rewrite <- (typ_subst_extend _ _ _ T1 H0 H').
+         rewrite <- (typ_subst_extend _ _ _ T2 H0 H').
          congruence.
-       apply* (unify_var _ _ _ _ _ _ R1 R2 H' H).
-       simpl; auto.
-      apply* (unify_var _ _ _ _ _ _ R1 R2 H' H).
+       unfold unify_vars in H.
+       remember (map (kind_subst S) K) as K0.
+       case_rewrite (get v K0) R3.
+       case_rewrite (get v0 K0) R4.
+       destruct (unify_kinds k k0).
+       assert (IS: is_subst (compose (v ~ typ_fvar v0) S)).
+         apply* add_binding_is_subst.
+         use (typ_subst_disjoint T2 H0).
+         rewrite R2 in H1.
+         disjoint_solve. simpl. destruct* (v1 == v). subst*.
+       rewrite <- (typ_subst_extend _ _ _ T1 IS H).
+       rewrite <- (typ_subst_extend _ _ _ T2 IS H).
+       use (typ_subst_disjoint T1 H0). rewrite  R1 in H1; simpl in H1.
+       repeat rewrite* typ_subst_compose; try (simpl; disjoint_solve).
+       rewrite R1; rewrite R2. simpl.
+       destruct* (v == v). destruct* (v0 == v).
+      apply* (unify_types_nv _ _ _ _ _ _ _ R1 R2 H' H).
      symmetry.
-     apply* (unify_var _ _ _ _ _ _ R2 R1 H' H).
-    rewrite <- (typ_subst_extend _ _ T1 H0 H').
-    rewrite <- (typ_subst_extend _ _ T2 H0 H').
+     apply* (unify_types_nv _ _ _ _ _ _ _ R2 R1 H' H).
+    rewrite <- (typ_subst_extend _ _ _ T1 H0 H').
+    rewrite <- (typ_subst_extend _ _ _ T2 H0 H').
     rewrite R1; rewrite R2.
     simpl.
-    rewrite* (IHh _ _ _ H H0 t t1).
-    rewrite* (IHh _ _ _ H H0 t0 t2).
+    rewrite* (IHh _ _ _ _ _ H H0 t t1).
+    rewrite* (IHh _ _ _ _ _ H H0 t0 t2).
   destruct p.
-  case_rewrite (typ_subst S0 t) R1; case_rewrite (typ_subst S0 t0) R2;
+  case_rewrite (typ_subst S t) R1; case_rewrite (typ_subst S t0) R2;
+    unfold unify_nv in H;
     try case_rewrite (S.mem v (typ_fv (typ_bvar n))) R3;
     try case_rewrite (S.mem v (typ_fv (typ_arrow t1 t2))) R3;
-    try apply* (IHh _ _ _ H);
+    fold kind in *;
+    try (case_rewrite (get v K) R4; destruct k; try discriminate);
+    try apply* (IHh _ _ _ _ _ H);
     try apply* add_binding_is_subst.
-        destruct (n === n0). subst. apply* (IHh _ _ _ H).
-        discriminate.
-       simpl; intro; auto.
+       destruct (n === n0). subst. apply* (IHh _ _ _ _ _ H).
+       discriminate.
       simpl; intro; auto.
-     destruct (v == v0).
-       subst.
-       apply* (IHh _ _ _ H).
-     apply* (IHh _ _ _ H).
-     apply* add_binding_is_subst.
-     use (typ_subst_disjoint t0 H0).
-     rewrite R2 in H2.
-     assert (v \notin typ_fv (typ_fvar v0)) by simpl*.
-     use (notin_disjoint H3).
-     disjoint_solve.
+     simpl; intro; auto.
+    destruct (v == v0).
+      subst.
+      apply* (IHh _ _ _ _ _ H).
+    unfold unify_vars in H.
+    remember (map (kind_subst S) K) as K0.
+    case_rewrite (get v K0) R3.
+    case_rewrite (get v0 K0) R4.
+    destruct (unify_kinds k k0).
+    apply* (IHh _ _ _ _ _ H).
+      apply* add_binding_is_subst.
+      use (typ_subst_disjoint t0 H0).
+      rewrite R2 in H2.
+      disjoint_solve.
+      simpl; destruct* (v1 == v). subst*.
+    apply* in_or_app.
    use (typ_subst_disjoint t0 H0).
    rewrite R2 in H2.
    use (notin_disjoint (mem_3 R3)).
@@ -383,6 +480,923 @@ Proof.
   rewrite R1 in H2.
   use (notin_disjoint (mem_3 R3)).
   disjoint_solve.
+Qed.
+
+Definition well_subst K K' S :=
+  forall Z k,
+    binds Z k K ->
+    well_kinded K' (kind_subst S k) (typ_subst S (typ_fvar Z)).
+
+Lemma well_kinded_subst: forall S K K' k T,
+  well_subst K K' S ->
+  well_kinded K k T ->
+  well_kinded K' (kind_subst S k) (typ_subst S T).
+Proof.
+  intros.
+  induction H0.
+    constructor.
+  generalize (H x _ H0); intro HW.
+  inversions HW.
+  simpl typ_subst.
+  case_eq (get x S); intros; rewrite H2 in H3.
+    subst.
+    simpl. apply* wk_kind.
+    apply* entails_trans.
+    apply* kind_subst_entails.
+  simpl.
+  inversions H3.
+  apply* wk_kind.
+  apply* entails_trans.
+  apply* kind_subst_entails.
+Qed.
+
+Section Accum.
+  Variables A B : Set.
+  Variables (f : A -> B) (op : B->B->B) (unit : B).
+
+  Fixpoint accum (l:list A) {struct l} : B :=
+    match l with
+    | nil => unit
+    | a::rem => op (f a) (accum rem)
+    end.
+End Accum.
+
+Fixpoint all_types S (pairs:list(typ*typ)) {struct pairs} : list typ :=
+  match pairs with
+  | nil => nil
+  | p::rem =>
+      typ_subst S (fst p) :: typ_subst S (snd p) :: all_types S rem
+  end.
+
+Definition all_fv S pairs :=
+  accum typ_fv S.union {} (all_types S pairs).
+Check all_fv.
+
+Lemma kind_subst_idem : forall S k,
+  is_subst S -> kind_subst S (kind_subst S k) = kind_subst S k.
+Proof.
+  intros.
+  destruct k as [[kc kr]|].
+    simpl.
+    apply (f_equal (fun kr => Some (Kind kc kr))).
+    induction kr; simpl. auto.
+    rewrite IHkr.
+    rewrite* typ_subst_idem.
+  auto.
+Qed.
+
+Lemma remove_notin : forall v L,
+  v \notin L -> S.remove v L = L.
+Proof.
+  intros.
+  apply eq_ext; intro; split; intro. eauto with sets.
+  apply* S.remove_2.
+  intro Hv; rewrite Hv in H; auto.
+Qed.
+
+Lemma remove_single : forall v, S.remove v {{v}} = {}.
+Proof.
+  intros; apply eq_ext; intros; split; intro.
+    use (S.remove_3 H).
+    elim (S.remove_1 (S.singleton_1 H0) H).
+  elim (in_empty H).
+Qed.
+
+Lemma dom_remove_env : forall (A:Set) v (K:Env.env A),
+  ok K ->
+ dom (remove_env K v) = S.remove v (dom K).
+Proof.
+  induction K; simpl; intros.
+    apply eq_ext; intros; split; intro. elim (in_empty H0).
+    apply* S.remove_3.
+  destruct a.
+  inversions H.
+  destruct (v == v0).
+    subst v0.
+    rewrite remove_union.
+    rewrite remove_single. rewrite* remove_notin. rewrite* union_empty_l.
+  simpl.
+  rewrite remove_union.
+  rewrite* IHK.
+  assert (v \notin {{v0}}) by auto.
+  rewrite* (remove_notin H0).
+Qed.
+
+Ltac union_solve x :=
+  match goal with
+  | H: x \in _ |- _ =>
+    destruct (S.union_1 H); clear H; auto with sets; try union_solve x
+  end.
+
+Lemma ok_remove_env : forall (A:Set) v (E:Env.env A),
+  ok E -> ok (remove_env E v).
+Proof.
+  induction E; simpl; intros. auto.
+  destruct a.
+  inversions H.
+  destruct* (v == v0).
+  apply* ok_cons.
+  clear -H4.
+  induction E; simpl. simpl in H4. auto.
+  destruct a.
+  simpl in H4.
+  destruct* (v == v1).
+  simpl. 
+  apply* notin_union_l.
+Qed.
+
+Hint Resolve ok_remove_env.
+
+Lemma typ_fv_decr : forall v T S T1,
+  v # S -> disjoint (typ_fv T) ({{v}} \u dom S) ->
+  typ_fv (typ_subst (compose (v ~ T) S) T1) <<
+  S.remove v (typ_fv T \u typ_fv (typ_subst S T1)).
+Proof.
+  intros.
+  rewrite* typ_subst_compose.
+  induction (typ_subst S T1); simpl in *; intros x Hx.
+      elim (in_empty Hx).
+    destruct (v0 == v).
+      subst.
+      apply* S.remove_2.
+        intro Hv; rewrite <- Hv in Hx. destruct* (H0 v).
+        elim H1; auto with sets.
+      auto with sets.
+    apply* S.remove_2.
+      intro Hv; rewrite <- Hv in Hx.
+      revert Hx; simpl*.
+    simpl in Hx; auto with sets.
+  destruct (S.union_1 Hx); [use (IHt1 _ H1) | use (IHt2 _ H1)];
+    apply* remove_subset;
+    intros y Hy; destruct (S.union_1 Hy); auto with sets.
+  simpl. intro x; destruct* (x == v).
+Qed.
+
+Lemma kind_fv_decr : forall v T S k,
+  v # S -> disjoint (typ_fv T) ({{v}} \u dom S) ->
+  kind_fv (kind_subst (compose (v ~ T) S) k) <<
+  S.remove v (typ_fv T \u kind_fv (kind_subst S k)).
+Proof.
+  intros.
+  unfold kind_fv.
+  destruct k as [[kc kr]|]; simpl.
+    induction kr; simpl; intros x Hx. elim (in_empty Hx).
+    destruct (S.union_1 Hx); clear Hx.
+      rewrite union_assoc.
+      rewrite remove_union.
+      use (typ_fv_decr _ _ _ H H0 H1). auto with sets.
+    rewrite union_assoc.
+    rewrite (union_comm (typ_fv T)).
+    rewrite <- union_assoc.
+    rewrite remove_union.
+    apply S.union_3. apply* IHkr.
+  intros x Hx; elim (in_empty Hx).
+Qed.
+
+Lemma fv_in_decr : forall (A:Set) v T S (E:Env.env A) fv (sub:subs -> A -> A),
+  v # S -> disjoint (typ_fv T) ({{v}} \u dom S) ->
+  (forall a,
+    fv (sub (compose (v ~ T) S) a) << S.remove v (typ_fv T \u fv (sub S a))) ->
+  fv_in fv (map (sub (compose (v ~ T) S)) E) <<
+  S.remove v (typ_fv T \u fv_in fv (map (sub S) E)).
+Proof.
+  intros.
+  induction E; intros x Hx; simpl in *. elim (in_empty Hx).
+  destruct a.
+  simpl in *.
+  destruct (S.union_1 Hx); clear Hx.
+    rewrite union_assoc.
+    rewrite remove_union.
+    apply S.union_2.
+    apply* (H1 a).
+  rewrite union_comm.
+  rewrite <- union_assoc.
+  rewrite remove_union.
+  apply S.union_3.
+  rewrite union_comm.
+  apply* IHE.
+Qed.
+
+Lemma all_fv_decr : forall v T S pairs,
+  v # S -> disjoint (typ_fv T) ({{v}} \u dom S) ->
+  all_fv (compose (v ~ T) S) pairs <<
+  S.remove v (all_fv S ((typ_fvar v, T) :: pairs)).
+Proof.
+  unfold all_fv.
+  induction pairs; intros.
+    simpl. intros x Hx. elim (in_empty Hx).
+  simpl.
+  intros x Hx.
+  rewrite* get_notin_dom.
+  destruct (S.union_1 Hx).
+    use (typ_fv_decr _ _ _ H H0 H1).
+    apply* remove_subset.
+    intros y Hy.
+    destruct (S.union_1 Hy).
+      rewrite <- (@typ_subst_fresh S T) in H3; auto with sets.
+      disjoint_solve.
+    auto with sets.
+  destruct (S.union_1 H1); clear Hx H1.
+    use (typ_fv_decr _ _ _ H H0 H2).
+    apply* remove_subset.
+    intros y Hy.
+    destruct (S.union_1 Hy).
+      rewrite <- (@typ_subst_fresh S T) in H3; auto with sets.
+      disjoint_solve.
+    auto with sets.
+  use (IHpairs H H0 _ H2).
+  apply* remove_subset.
+  simpl.
+  rewrite* get_notin_dom.
+  intros y Hy.
+  clear H1 H2.
+  simpl in Hy.
+  destruct (S.union_1 Hy). auto with sets.
+  destruct (S.union_1 H1); auto with sets.
+Qed.
+
+Definition id := Env.empty (A:=typ).
+
+Lemma typ_subst_id : forall T, typ_subst id T = T.
+Proof.
+  intro.
+  apply typ_subst_fresh.
+  simpl. intro; auto.
+Qed.
+
+Lemma is_subst_id : is_subst id.
+Proof.
+  unfold id, is_subst. intro; intros. elim (binds_empty H).
+Qed.
+
+Definition really_all_fv S K pairs :=
+  fv_in kind_fv (map (kind_subst S) K) \u all_fv S pairs.
+
+Lemma really_all_fv_decr : forall S K t t0 pairs v T,
+  really_all_fv S K ((t, t0) :: pairs) \u fv_in typ_fv S << dom K ->
+  typ_subst S t = typ_fvar v ->
+  typ_subst S t0 = T ->
+  is_subst S ->
+  ok K ->
+  S.mem v (typ_fv T) = false ->
+  really_all_fv (compose (v ~ T) S) (remove_env K v) pairs \u
+  fv_in typ_fv (compose (v ~ T) S) << S.remove v (dom K).
+Proof.
+  intros until T. intros Hra R1 R2 HS HK R3.
+  unfold really_all_fv in *.
+  intros x Hx.
+  apply* remove_subset.
+  clear Hra.
+  assert (v # S) by apply* typ_subst_res_fresh.
+  assert (disjoint (typ_fv T) ({{v}} \u dom S)).
+    use (typ_subst_disjoint t0 HS). rewrite R2 in H0.
+    disjoint_solve.
+    destruct* (v0 == v); subst*.
+  destruct (S.union_1 Hx); clear Hx.
+    rewrite remove_union; apply S.union_2.
+    destruct (S.union_1 H1); clear H1.
+      unfold all_fv; simpl. rewrite R2.
+      rewrite (union_comm (typ_fv (typ_subst S t))).
+      do 2 rewrite union_assoc. do 2 (rewrite remove_union; apply S.union_2).
+      rewrite union_comm.
+      refine (fv_in_decr _ _ _ _ _ _ _ _ _); auto.
+      intros; apply* kind_fv_decr.
+      clear -H2; induction K; simpl in *. auto.
+      destruct a; simpl.
+      destruct (v == v0); simpl in H2.
+        auto with sets.
+      destruct (S.union_1 H2); auto with sets.
+    rewrite remove_union; apply S.union_3.
+    unfold all_fv; simpl.
+    rewrite <- (typ_subst_idem t HS).
+    rewrite <- (typ_subst_idem t0 HS).
+    rewrite R1; rewrite R2.
+    apply (all_fv_decr _ _ _ H H0 H2).
+  unfold all_fv; simpl. rewrite R2.
+  rewrite (union_comm (typ_fv T)).
+  do 3 rewrite <- union_assoc.
+  do 3 (rewrite remove_union; apply S.union_3).
+  unfold compose in H1.
+  simpl in H1.
+  destruct (S.union_1 H1).
+    rewrite remove_union.
+    rewrite remove_notin. auto with sets.
+    destruct* (H0 v).
+  replace S with (map (typ_subst id) S).
+    replace (v~T) with (compose (v~T) id) in H2.
+      assert (v # id) by (unfold id; auto).
+      assert (disjoint (typ_fv T) ({{v}} \u dom id))
+        by (simpl; disjoint_solve).
+      refine (fv_in_decr _ _ _ _ _ _ _ _ _); auto.
+      intros; apply* typ_fv_decr.
+    reflexivity.
+  clear; induction S; simpl; auto.
+  destruct a; simpl; rewrite typ_subst_id; rewrite* IHS.
+Qed.
+
+Lemma really_all_fv_comm : forall S K t t0 pairs,
+  really_all_fv S K ((t,t0)::pairs) = really_all_fv S K ((t0,t)::pairs).
+Proof.
+  intros.
+  unfold really_all_fv, all_fv; simpl.
+  rewrite (union_assoc (typ_fv (typ_subst S t))).
+  rewrite (union_comm (typ_fv (typ_subst S t))).
+  rewrite* <- (union_assoc (typ_fv (typ_subst S t0))).
+Qed.
+
+Lemma binds_remove_env : forall (A:Set) v K x (a:A),
+  binds x a K -> x <> v -> binds x a (remove_env K v).
+Proof.
+  unfold binds; induction K; simpl; intros. auto.
+  destruct a; simpl in *.
+  destruct (x == v0).
+    destruct (v == v0). subst. elim H0; auto.
+    simpl. destruct* (x == v0).
+  destruct* (v == v0).
+  simpl. destruct* (x == v0).
+Qed.
+
+Lemma kind_subst_combine : forall S S1 S2 k,
+  (forall T, typ_subst S1 (typ_subst S2 T) = typ_subst S T) ->
+  kind_subst S1 (kind_subst S2 k) = kind_subst S k.
+Proof.
+  intros.
+  destruct k as [[kc kr]|].
+    simpl.
+    apply (f_equal (fun kr => Some (Kind kc kr))).
+    induction kr. auto.
+    simpl. rewrite IHkr. rewrite* H.
+  auto.
+Qed.
+
+Definition unify_kinds_spec pairs K S K' S' :=
+  is_subst S -> ok K ->
+  disjoint (dom S) (dom K) ->
+  really_all_fv S K pairs \u fv_in typ_fv S << dom K ->
+  ok K' /\ disjoint (dom S') (dom K') /\
+  fv_in kind_fv (map (kind_subst S') K') \u fv_in typ_fv S' << dom K' /\
+  well_subst (map (kind_subst S) K) (map (kind_subst S') K') S'.
+
+Lemma unify_kinds_nv : forall h pairs K S v T K' S' h' pairs' t t0,
+  unify_nv (unify h pairs) K S v T = Some (K', S') ->
+  typ_subst S t = typ_fvar v ->
+  typ_subst S t0 = T ->
+  unify h' pairs' K S = Some (K',S') ->
+  (forall pairs K S,
+    unify h pairs K S = Some (K',S') -> unify_kinds_spec pairs K S K' S') ->
+  unify_kinds_spec ((t,t0)::pairs) K S K' S'.
+Proof.
+  unfold unify_nv.
+  intros until 1.
+  intros R1 R2 H' IHh HS Hk Dis Hra.
+  case_rewrite (S.mem v (typ_fv T)) R3.
+  case_rewrite (get v K) R4.
+  destruct o. discriminate.
+  assert (His : is_subst (compose (v ~ T) S)).
+    apply* add_binding_is_subst.
+    use (typ_subst_disjoint t0 HS).
+    rewrite R2 in H0.
+    use (notin_disjoint (mem_3 R3)).
+    disjoint_solve.
+  destruct* (IHh _ _ _ H); clear IHh.
+      rewrite* dom_remove_env.
+      unfold compose. simpl.
+      rewrite dom_map.
+      intro x; destruct (v == x).
+        right; apply* S.remove_1.
+      destruct* (Dis x). right; intro. elim H0; apply* S.remove_3.
+    rewrite* dom_remove_env.
+    apply* really_all_fv_decr.
+  intuition.
+  intro; intros.
+  unfold well_subst in H4.
+  destruct (binds_map_inv _ _ H3) as [k0 [Hk0 B]].
+  destruct (Z == v).
+    subst. fold kind in R4. rewrite B in R4.
+    inversions R4. simpl. apply wk_any.
+  use (binds_map (kind_subst (compose (v ~ T) S)) (binds_remove_env B n)).
+  use (H4 _ _ H5).
+  rewrite (@kind_subst_combine S') in H6.
+    rewrite <- (@kind_subst_combine S' S' S) in H6.
+      rewrite Hk0 in H6. auto.
+    intro; apply* typ_subst_extend.
+  intro; apply* typ_subst_extend.
+Qed.
+
+Lemma in_all_fv : forall S t t0 l,
+  In (t,t0) l ->
+  typ_fv (typ_subst S t) \u typ_fv (typ_subst S t0) << all_fv S l.
+Proof.
+  induction l; simpl; intros H x Hx. elim H.
+  unfold all_fv; simpl.
+  destruct H.
+    subst; simpl.
+    rewrite union_assoc; auto with sets.
+  rewrite union_assoc; apply S.union_3; apply* IHl.
+Qed.
+
+Lemma in_typ_fv : forall t l,
+  In t l -> typ_fv t << typ_fv_list l.
+Proof.
+  induction l; simpl; intros H x Hx. elim H.
+  destruct H.
+    subst; simpl.
+    auto with sets.
+  apply S.union_3; apply* IHl.
+Qed.
+
+Lemma unify_kinds_fv : forall k k0 k1 l S,
+  unify_kinds k k0 = (k1, l) ->
+  kind_fv (kind_subst S k1) \u all_fv S l <<
+  kind_fv (kind_subst S k) \u kind_fv (kind_subst S k0).
+Proof.
+  unfold unify_kinds; intros.
+  destruct k as [[kc kr]|].
+    destruct k0 as [[kc0 kr0]|].
+      case_rewrite
+        (unify_kind_rel (kr ++ kr0) nil (unique (cstr_lub kc kc0)) nil) R1.
+      inversions H; clear H. simpl.
+      unfold kind_fv; simpl.
+      repeat rewrite map_map; simpl.
+      rewrite <- fv_list_map. rewrite <- map_app.
+      set (pairs := nil(A:=typ*typ)) in *.
+      set (kr' := nil(A:=var*typ)) in *.
+      intros x Hx.
+      rewrite <- union_empty_r.
+      replace {} with
+        (typ_fv_list (List.map (fun x : var * typ => typ_subst S (snd x)) kr'))
+        by reflexivity.
+      rewrite <- union_empty_r.
+      replace {} with (all_fv S pairs) by reflexivity.
+      clearbody pairs kr'.
+      gen pairs kr'; induction (kr ++ kr0); simpl; intros.
+        inversions R1; intuition.
+        rewrite <- union_assoc; auto with sets.
+      destruct a; simpl.
+      destruct (In_dec eq_var_dec v (unique (cstr_lub kc kc0))).
+        case_rewrite (get v kr') R2; poses Hsub (IHl1 _ _ R1).
+          rewrite <- union_assoc in Hsub.
+          destruct (S.union_1 Hsub); clear Hsub; auto with sets.
+          destruct (S.union_1 H); clear H; auto with sets.
+          unfold all_fv in H0; simpl in H0.
+          destruct (S.union_1 H0); clear H0; auto with sets.
+          destruct (S.union_1 H); clear H; auto with sets.
+Lemma get_in : forall (A:Set) x (a:A) E,
+  binds x a E -> In (x, a) E.
+Proof.
+  unfold binds; induction E; intros. elim (binds_empty H).
+  destruct a0; simpl in *.
+  destruct* (x == v). inversions* H.
+Qed.
+          use (get_in R2).
+          use (in_map (fun x : var * typ => typ_subst S (snd x)) _ _ H).
+          use (in_typ_fv _ _ H1 H0).
+          auto with sets.
+        simpl in Hsub. union_solve x.
+      poses Hsub (IHl1 _ _ R1); clear IHl1 Hx.
+      simpl in Hsub.
+      union_solve x.
+    inversions H.
+    unfold kind_fv, all_fv; simpl.
+    apply subset_refl.
+  inversions H.
+  unfold kind_fv, all_fv; simpl.
+  rewrite union_comm; apply subset_refl.
+Qed.
+
+Definition kind_entails k k' :=
+  match k', k with
+  | None, _ => True
+  | Some c', Some c => entails c c'
+  |  Some c', None => False
+  end.
+
+Lemma unify_kind_rel_keep : forall kr kr' un pairs k' l,
+  unify_kind_rel kr kr' un pairs = (k', l) ->
+  incl kr' k' /\ incl pairs l.
+Proof.
+  induction kr; simpl; intros. inversions H. split*.
+  destruct a.
+  destruct (In_dec eq_var_dec v un).
+    case_rewrite (get v kr') R1; destruct* (IHkr _ _ _ _ _ H).
+  destruct* (IHkr _ _ _ _ _ H).
+Qed.
+
+Lemma well_subst_unify_kinds : forall k k0 k1 l S,
+  unify_kinds k k0 = (k1, l) ->
+  (forall T1 T2, In (T1, T2) l -> typ_subst S T1 = typ_subst S T2) ->
+  kind_entails (kind_subst S k1) (kind_subst S k) /\
+  kind_entails (kind_subst S k1) (kind_subst S k0).
+Proof.
+  unfold unify_kinds, kind_entails.
+  intros.
+  destruct k as [[kc kr]|]; destruct k0 as [[kc0 kr0]|]; simpl.
+     case_rewrite
+       (unify_kind_rel (kr ++ kr0) nil (unique (cstr_lub kc kc0)) nil) R1.
+     inversions H; clear H.
+     simpl.
+     assert (incl
+       (List.map (fun XT : var * typ => (fst XT, typ_subst S (snd XT)))
+         (kr ++ kr0))
+       (List.map (fun XT : var * typ => (fst XT, typ_subst S (snd XT))) l0)).
+       clear -H0 R1.
+       set (pairs := nil(A:=typ*typ)) in R1.
+       set (kr' := nil(A:=var*typ)) in R1.
+       clearbody pairs kr'.
+       intros T HT.
+       destruct T; gen kr' pairs; induction (kr++kr0); simpl; intros. elim HT.
+       destruct a.
+       destruct (In_dec eq_var_dec v0 (unique (cstr_lub kc kc0)));
+         try case_rewrite (get v0 kr') R2; simpl in HT; destruct HT;
+         try solve [apply* IHl1]; inversions H; clear H;
+         destruct (unify_kind_rel_keep _ _ _ _ R1).
+           use (H _ (get_in R2)); clear H.
+           assert (In (t0,t1) l) by auto.
+           use (H0 _ _ H).
+           rewrite H3.
+           refine (in_map _ _ _ H2).
+         assert (In (v,t0) l0) by auto.
+         refine (in_map _ _ _ H2).
+       assert (In (v,t0) l0) by auto.
+       refine (in_map _ _ _ H2).
+     destruct (proj2 (cstr_lub_ok kc kc0 _) (Cstr.entails_refl _)).
+     split; split*; simpl; intros; apply H; rewrite map_app; apply* in_or_app.
+    split*.
+    inversions H; clear H.
+    simpl. apply entails_refl.
+   split*.
+   inversions H; clear H.
+   simpl. apply entails_refl.
+  auto.
+Qed.
+
+Lemma all_fv_app : forall S l1 l2,
+  all_fv S (l1 ++ l2) = all_fv S l1 \u all_fv S l2.
+Proof.
+  intros.
+  unfold all_fv.
+  induction l1; simpl. rewrite* union_empty_l.
+  rewrite IHl1.
+  repeat rewrite union_assoc. auto.
+Qed.
+
+Lemma map_remove_env : forall (A:Set) x f (E:Env.env A),
+  map f (remove_env E x) = remove_env (map f E) x.
+Proof.
+  induction E; simpl in *. auto.
+  destruct a; simpl.
+  destruct (x == v); simpl*.
+  rewrite* IHE.
+Qed.
+
+Lemma map_map_env : forall (A:Set) f f1 f2 (E:Env.env A),
+  (forall x, f x = f1 (f2 x)) -> map f E = map f1 (map f2 E).
+Proof.
+  intros; induction E; simpl. auto.
+  destruct a; simpl.
+  rewrite H.
+  rewrite* IHE.
+Qed.
+
+Lemma fv_in_remove_env : forall (A:Set) (fv:A->vars) x E,
+  fv_in fv (remove_env E x) << fv_in fv E.
+Proof.
+  induction E; simpl. apply subset_refl.
+  destruct a; simpl.
+  destruct (x == v); simpl; intros y Hy; auto with sets.
+  destruct (S.union_1 Hy). auto with sets.
+  use (IHE _ H). auto with sets.
+Qed.
+
+Lemma well_subst_unify : forall k k0 k1 l v v0 S K SK S' K' h pairs h' pairs',
+  unify h (l ++ pairs) (remove_env (remove_env SK v) v0 & v0 ~ k1)
+    (compose (v ~ typ_fvar v0) S) = Some (K', S') ->
+  unify h' pairs' K S = Some (K', S') ->
+  unify_kinds k k0 = (k1, l) ->
+  SK = map (kind_subst S) K ->
+  binds v k SK ->
+  binds v0 k0 SK ->
+  is_subst S ->
+  is_subst (compose (v ~ typ_fvar v0) S) ->
+  v # S ->
+  v <> v0 ->
+  well_subst
+    (map (kind_subst (compose (v ~ typ_fvar v0) S))
+      (remove_env (remove_env SK v) v0 & v0 ~ k1))
+    (map (kind_subst S') K') S' ->
+  well_subst SK (map (kind_subst S') K') S'.
+Proof.
+  intros until 1; intros H' HU HeqSK B1 B2 HS HS1 Hv n WS x; intros.
+  unfold well_subst in WS.
+  use (fun T => typ_subst_extend _ _ _ T HS1 H).
+  use (unify_types _ _ _ H HS1).
+  destruct (x == v0).
+    subst.
+    rewrite (binds_func H0 B2) in *; clear H0.
+    assert (well_kinded (map (kind_subst S') K') (kind_subst S' k1)
+               (typ_subst S' (typ_fvar v0))).
+      rewrite <- (kind_subst_combine S' S' (compose (v ~ typ_fvar v0) S)).
+      apply WS. apply binds_map. apply binds_head. auto.
+    use (proj1 (unify_keep _ _ _ H HS1)).
+    use (unify_types _ _ _ H HS1).
+    assert (forall T1 T2 : typ, In (T1, T2) l ->
+               typ_subst S' T1 = typ_subst S' T2).
+      intros. apply H4. apply* in_or_app.
+    destruct (well_subst_unify_kinds _ _ S' HU H5).
+    clear H4 H5 H6.
+    inversions H0.
+      rewrite <- H6 in H7.
+      unfold kind_entails in H7; simpl in H7.
+      case_rewrite (kind_subst S' k0) R4. elim H7.
+      apply wk_any.
+    simpl; rewrite <- H5.
+    rewrite <- H4 in H7.
+    unfold kind_entails in H7; simpl in H7.
+    case_rewrite (kind_subst S' k0) R4.
+      apply* wk_kind. apply* entails_trans.
+    apply wk_any.
+  destruct (x == v).
+    subst.
+    rewrite (binds_func H0 B1) in *; clear H0.
+    use (proj1 (unify_keep _ _ _ H HS1)).
+    assert (well_kinded (map (kind_subst S') K') (kind_subst S' k1)
+               (typ_subst S' (typ_fvar v))).
+      rewrite <- (kind_subst_combine S' S' (compose (v ~ typ_fvar v0) S)).
+      rewrite <- (typ_subst_extend _ _ _ (typ_fvar v) HS1 H).
+      destruct (binds_map_inv _ _ B1).
+      rewrite* typ_subst_compose.
+      rewrite* (typ_subst_fresh S).
+      simpl. destruct* (v == v).
+      simpl. intro y; destruct* (y == v).
+      simpl. intro y; destruct* (y == v).
+      intros. apply* typ_subst_extend.
+    use (unify_types _ _ _ H HS1).
+    assert (forall T1 T2 : typ, In (T1, T2) l ->
+               typ_subst S' T1 = typ_subst S' T2).
+      intros. apply H4. apply* in_or_app.
+    destruct (well_subst_unify_kinds _ _ S' HU H5).
+    clear H4 H5 H7.
+    inversions H3.
+      rewrite <- H7 in H6.
+      unfold kind_entails in H6; simpl in H6.
+      case_rewrite (kind_subst S' k) R4. elim H6.
+      apply wk_any.
+    simpl; rewrite <- H5.
+    rewrite <- H4 in H6.
+    unfold kind_entails in H6; simpl in H6.
+    case_rewrite (kind_subst S' k) R4.
+      apply* wk_kind. apply* entails_trans.
+    apply wk_any.
+  subst.
+  assert (x # v0 ~ k1) by simpl*.
+  use (binds_map (kind_subst (compose (v ~ typ_fvar v0) S))
+          (binds_concat_fresh _ (binds_remove_env (binds_remove_env H0 n1) n0)
+            H3)).
+  use (WS _ _ H4).
+  rewrite (@kind_subst_combine S') in H5. auto.
+  intro; apply* typ_subst_extend.
+Qed.
+
+Lemma unify_kinds_vars :
+  forall h pairs K S v v0 K' S' h' pairs' t t0 k k0 k1 l SK,
+  unify h (l ++ pairs) (remove_env (remove_env SK v) v0 & v0 ~ k1)
+    (compose (v ~ typ_fvar v0) S) = Some (K', S') ->
+  typ_subst S t = typ_fvar v ->
+  typ_subst S t0 = typ_fvar v0 ->
+  v <> v0 ->
+  SK = map (kind_subst S) K ->
+  binds v k SK ->
+  binds v0 k0 SK ->
+  unify_kinds k k0 = (k1, l) ->
+  unify h' pairs' K S = Some (K',S') ->
+  (forall pairs K S,
+    unify h pairs K S = Some (K',S') -> unify_kinds_spec pairs K S K' S') ->
+  unify_kinds_spec ((t,t0)::pairs) K S K' S'.
+Proof.
+  intros until SK.
+  intros H R1 R2 n HeqSK R3 R4 R5 H' IHh HS HK Dis Hra.
+  assert (His: is_subst (compose (v ~ typ_fvar v0) S)).
+    apply* add_binding_is_subst.
+    use (typ_subst_disjoint t0 HS).
+    rewrite R2 in H0.
+    simpl in *.
+    intro x. destruct* (x == v0). subst v0; destruct* (H0 x).
+  assert (HSK: ok SK).
+    rewrite (app_nil_end SK).
+    fold (nil & SK).
+    rewrite HeqSK. apply ok_map.
+    unfold concat; rewrite* <- (app_nil_end K).
+  destruct* (IHh _ _ _ H); clear IHh.
+        constructor. repeat apply ok_remove_env. auto.
+        rewrite dom_remove_env.
+          apply S.remove_1. reflexivity.
+        apply* ok_remove_env.
+      simpl.
+      rewrite dom_map.
+      repeat rewrite* dom_remove_env.
+      disjoint_solve.
+        destruct* (v1 == v).
+        subst; right.
+        apply* notin_union_l.
+        intro.
+        use (S.remove_3 H1).
+        elim (S.remove_1 (refl_equal v) H2).
+      destruct* (v1 == v0).
+        subst; left.
+        use (typ_subst_res_fresh _ HS R2).
+      right; apply* notin_union_l.
+      intro.
+      use (S.remove_3 (S.remove_3 H1)).
+      rewrite HeqSK in H2.
+      rewrite dom_map in H2. auto.
+    assert (S.mem v (typ_fv (typ_fvar v0)) = false).
+      simpl. case_eq (S.mem v {{v0}}); intros; auto.
+      pose (S.mem_2 H0).
+      elim n; rewrite* (S.singleton_1 i).
+    poses Hsub (really_all_fv_decr Hra R1 R2 HS HK H0).
+    intros x Hx.
+    unfold really_all_fv in Hx.
+    rewrite all_fv_app in Hx.
+    simpl in Hx.
+    repeat rewrite union_assoc in Hx.
+    simpl.
+    rewrite* dom_remove_env.
+    destruct (x == v0). subst; auto with sets.
+    rewrite* dom_remove_env.
+    rewrite HeqSK; rewrite dom_map.
+    assert (v # S) by apply* typ_subst_res_fresh.
+    assert (disjoint (typ_fv (typ_fvar v0)) ({{v}} \u dom S)).
+      simpl; intro y; destruct* (y == v0); subst.
+      use (typ_subst_res_fresh _ HS R2).
+    assert (forall y k,
+              binds y k SK ->
+              x \in kind_fv (kind_subst (compose (v ~ typ_fvar v0) S) k) ->
+              x \in {{v0}} \u S.remove v0 (S.remove v (dom K))).
+      clear Hx; intros.
+      use (kind_fv_decr _ _ _ H1 H2 H4).
+      simpl in H5; rewrite remove_union in H5.
+      destruct (S.union_1 H5); clear H4 H5.
+        apply S.union_2; apply* S.remove_3.
+      apply S.union_3; apply* S.remove_2.
+      apply S.remove_2. intro Hv; elim (S.remove_1 Hv H6).
+      apply Hra.
+      unfold really_all_fv.
+      repeat apply S.union_2.
+      use (S.remove_3 H6).
+      rewrite <- HeqSK.
+      apply (fv_in_spec kind_fv H3).
+      rewrite HeqSK in H3.
+      destruct (binds_map_inv _ _ H3) as [k' [E B]].
+      subst.
+      rewrite kind_subst_idem in H4; auto.
+    union_solve x.
+            poses Hfv (unify_kinds_fv _ _ _ R5 (S.union_2 _ H4)); clear H4.
+            destruct (S.union_1 Hfv); clear Hfv. apply* (H3 _ _ R3 H4).
+            apply* H3.
+          apply S.union_3.
+          apply S.remove_2. intro Hx; elim n0; rewrite* Hx.
+          apply Hsub.
+          apply S.union_2.
+          clear H H' Hsub Hra; unfold really_all_fv in *.
+          apply S.union_2.
+          subst.
+          repeat rewrite map_remove_env in *.
+          rewrite <- (map_map_env (kind_subst (compose (v ~ typ_fvar v0) S)))
+            in H4.
+            apply (fv_in_remove_env _ _ _ H4).
+          intro.
+          rewrite (kind_subst_combine (compose (v ~ typ_fvar v0) S)). auto.
+          intro.
+          assert (disjoint (dom (v ~ typ_fvar v0)) (dom S)).
+            simpl. use (typ_subst_res_fresh _ HS R1).
+            intro y; destruct* (y == v).
+          repeat rewrite* typ_subst_compose. rewrite* typ_subst_idem.
+        poses Hfv (unify_kinds_fv _ _ _ R5 (S.union_3 _ H5)).
+        destruct (S.union_1 Hfv); clear Hfv. apply* (H3 _ _ R3 H4).
+        apply* H3.
+      unfold really_all_fv in Hsub.
+      apply S.union_3.
+      apply S.remove_2. intro Hx; elim n0; rewrite* Hx.
+      apply Hsub; clear H H' Hra Hsub.
+      auto with sets.
+    unfold really_all_fv in Hsub.
+    apply S.union_3.
+    apply S.remove_2. intro Hx; elim n0; rewrite* Hx.
+    apply Hsub; clear H H' Hra Hsub.
+    unfold compose. simpl.
+    auto with sets.
+  intuition.
+  subst; apply* well_subst_unify.
+  apply* typ_subst_res_fresh.
+Qed.
+
+Theorem unify_kinds_ok : forall h pairs K S K' S',
+  unify h pairs K S = Some (K',S') ->
+  unify_kinds_spec pairs K S K' S'.
+Proof.
+  induction h; intros; intros HS Hk Dis Hra. discriminate.
+  poses H' H.
+  simpl in H.
+  destruct pairs.
+    inversions H.
+    intuition.
+      intros x Hx; apply Hra.
+      unfold really_all_fv.
+      destruct (S.union_1 Hx); auto with sets.
+    intro; intros.
+    destruct (binds_map_inv _ _ H0) as [k0 [HE B]].
+    subst.
+    rewrite* typ_subst_fresh.
+      rewrite* kind_subst_idem.
+      destruct k0.
+        simpl in *. apply* wk_kind.
+        split; simpl*.
+      apply wk_any.
+    case_eq (S.mem Z (dom K')); intros.
+      use (S.mem_2 H1).
+      destruct* (Dis Z).
+      intro. destruct* (x == Z). simpl*.
+    elim (binds_fresh B (mem_3 H1)).
+  destruct p.
+  case_rewrite (typ_subst S t) R1; case_rewrite (typ_subst S t0) R2.
+        destruct (n === n0).
+          apply* (IHh _ _ _ _ _ H).
+          intros x Hx; apply Hra.
+          clear -Hx.
+          unfold really_all_fv, all_fv in *; simpl.
+          union_solve x.
+        discriminate.
+       rewrite really_all_fv_comm in Hra.
+       refine (unify_kinds_nv h _ _ H R2 R1 H' _ _ _ _ _); auto.
+      refine (unify_kinds_nv h _ _ H R1 R2 H' _ _ _ _ _); auto.
+      destruct (v == v0).
+        subst.
+        apply* (IHh _ _ _ _ _ H).
+        intros x Hx; apply Hra.
+        clear -Hx.
+        unfold really_all_fv, all_fv in *; simpl.
+        union_solve x.
+      unfold unify_vars in H.
+      remember (map (kind_subst S) K) as SK.
+      case_rewrite (get v SK) R3.
+      case_rewrite (get v0 SK) R4.
+      case_rewrite (unify_kinds k k0) R5.
+      subst; refine (unify_kinds_vars _ _ _ H R1 R2 n _ R3 R4 R5 H' _ _ _ _ _);
+        auto.
+     refine (unify_kinds_nv h _ _ H R1 R2 H' _ _ _ _ _); auto.
+    rewrite really_all_fv_comm in Hra.
+    refine (unify_kinds_nv h _ _ H R2 R1 H' _ _ _ _ _); auto.
+  destruct* (IHh _ _ _ _ _ H HS).
+  clear -Hra R1 R2 HS.
+  unfold really_all_fv, all_fv in *; simpl in *.
+  intros x Hx; apply Hra; clear Hra.
+  rewrite <- (typ_subst_idem t HS).
+  rewrite <- (typ_subst_idem t0 HS).
+  rewrite R1; rewrite R2.
+  simpl.
+  repeat rewrite <- union_assoc in *.
+  union_solve x.
+Qed.
+       
+Lemma typ_subst_map_idem : forall S,
+  is_subst S -> ok S -> map (typ_subst S) S = S.
+Proof.
+  intros.
+  remember S as S0.
+  pattern S0 at 1.
+  rewrite HeqS0.
+  assert (env_prop (fun T => typ_subst S T = T) S0).
+    intro; intros.
+    rewrite <- HeqS0.
+    rewrite <- (binds_typ_subst H1).
+    apply* typ_subst_idem.
+  clear HeqS0 H.
+  induction S0. auto.
+  inversions H0.
+  simpl. rewrite (H1 x a0).
+    rewrite* IHS0.
+    intro; intros.
+    apply (H1 x0 a).
+    unfold binds. simpl.
+    destruct* (x0 == x).
+    subst. elim (binds_fresh H H4).
+  unfold binds; simpl.
+  destruct* (x == x).
+Qed.
+
+Lemma fv_in_subset_inv : forall (A:Set) fv F E,
+  fv_in fv E << F <-> forall x (a:A), In (x,a) E -> fv a << F.
+Proof.
+  induction E; intros; split; intros. elim H0.
+      simpl. intros x Hx; elim (in_empty Hx).
+    simpl in *; destruct H0.
+      subst.
+      destruct* (proj1 (subset_union_l (fv a0) (fv_in fv E) F)).
+    destruct a.
+    destruct* (proj1 (subset_union_l (fv a) (fv_in fv E) F)).
+  simpl in *.
+  destruct a.
+  apply* (proj2 (subset_union_l (fv a) (fv_in fv E) F)).
 Qed.
 
 Lemma typ_subst_prebind : forall v T S T1,
@@ -398,15 +1412,6 @@ Proof.
   rewrite* IHT1_1. rewrite* IHT1_2.
 Qed.
 
-Lemma typ_subst_res_fresh : forall S T v,
-  is_subst S -> typ_subst S T = typ_fvar v -> v # S.
-Proof.
-  intros.
-  use (typ_subst_disjoint T H).
-  rewrite H0 in H1.
-  simpl in H1. destruct* (H1 v).
-Qed.
-
 Definition mgu_spec pairs S0 S S' :=
   is_subst S0 ->
   (forall T1 T2, In (T1,T2) pairs ->
@@ -418,7 +1423,7 @@ Definition mgu_spec pairs S0 S S' :=
 Lemma unify_mgu_step : forall S0 pairs S S' h t t0 v T,
   typ_subst S0 t = typ_fvar v ->
   typ_subst S0 t0 = T ->
-  unify pairs (add_binding v T S0) h = Some S ->
+  unify pairs (compose (v ~ T) S0) h = Some S ->
   S.mem v (typ_fv T) = false ->
   (forall S0, unify pairs S0 h = Some S -> mgu_spec pairs S0 S S') ->
   mgu_spec ((t,t0)::pairs) S0 S S'.
@@ -432,8 +1437,8 @@ Proof.
     rewrite R1 in H1; rewrite R2 in H1.
     auto.
   assert (Hv: v # S0) by apply* typ_subst_res_fresh.
-  assert (typ_subst S' (typ_subst (add_binding v T S0) T1) =
-          typ_subst S' (typ_subst (add_binding v T S0) T2)).
+  assert (typ_subst S' (typ_subst (compose (v ~ T) S0) T1) =
+          typ_subst S' (typ_subst (compose (v ~ T) S0) T2)).
     apply* IHh.
       apply* add_binding_is_subst.
       assert (disjoint {{v}} (typ_fv T)).
@@ -495,20 +1500,6 @@ Proof.
   destruct* H3. inversions* H3.
 Qed.
 
-Definition id := Env.empty (A:=typ).
-
-Lemma typ_subst_id : forall T, typ_subst id T = T.
-Proof.
-  intro.
-  apply typ_subst_fresh.
-  simpl. intro; auto.
-Qed.
-
-Lemma is_subst_id : is_subst id.
-Proof.
-  unfold id, is_subst. intro; intros. elim (binds_empty H).
-Qed.
-
 Theorem unify_mgu : forall h S S' T1 T2,
   unify ((T1,T2)::nil) id h = Some S ->
   typ_subst S' T1 = typ_subst S' T2 ->
@@ -526,28 +1517,6 @@ Proof.
   repeat rewrite typ_subst_id.
   auto.
 Qed.
-
-Section Accum.
-  Variables A B : Set.
-  Variables (f : A -> B) (op : B->B->B) (unit : B).
-
-  Fixpoint accum (l:list A) {struct l} : B :=
-    match l with
-    | nil => unit
-    | a::rem => op (f a) (accum rem)
-    end.
-End Accum.
-
-Fixpoint all_types S (pairs:list(typ*typ)) {struct pairs} : list typ :=
-  match pairs with
-  | nil => nil
-  | p::rem =>
-      typ_subst S (fst p) :: typ_subst S (snd p) :: all_types S rem
-  end.
-
-Definition all_fv S pairs :=
-  accum typ_fv S.union {} (all_types S pairs).
-Check all_fv.
 
 Fixpoint typ_size (T : typ) : nat :=
   match T with
@@ -607,71 +1576,9 @@ Proof.
   omega.
 Qed.
 
-Lemma typ_fv_decr : forall v T S T1,
-  v # S -> disjoint (typ_fv T) ({{v}} \u dom S) ->
-  typ_fv (typ_subst (add_binding v T S) T1) <<
-  S.remove v (typ_fv T \u typ_fv (typ_subst S T1)).
-Proof.
-  intros.
-  rewrite* typ_subst_add_binding.
-  induction (typ_subst S T1); simpl in *; intros x Hx.
-      elim (in_empty Hx).
-    destruct (v0 == v).
-      subst.
-      apply* S.remove_2.
-        intro Hv; rewrite <- Hv in Hx. destruct* (H0 v).
-        elim H1; auto with sets.
-      auto with sets.
-    apply* S.remove_2.
-      intro Hv; rewrite <- Hv in Hx.
-      revert Hx; simpl*.
-    simpl in Hx; auto with sets.
-  destruct (S.union_1 Hx); [use (IHt1 _ H1) | use (IHt2 _ H1)];
-    apply* remove_subset;
-    intros y Hy; destruct (S.union_1 Hy); auto with sets.
-Qed.
-
-Lemma all_fv_decr : forall v T S pairs,
-  v # S -> disjoint (typ_fv T) ({{v}} \u dom S) ->
-  all_fv (add_binding v T S) pairs <<
-  S.remove v (all_fv S ((typ_fvar v, T) :: pairs)).
-Proof.
-  unfold all_fv.
-  induction pairs; intros.
-    simpl. intros x Hx. elim (in_empty Hx).
-  simpl.
-  intros x Hx.
-  rewrite* get_notin_dom.
-  destruct (S.union_1 Hx).
-    use (typ_fv_decr _ _ _ H H0 H1).
-    apply* remove_subset.
-    intros y Hy.
-    destruct (S.union_1 Hy).
-      rewrite <- (@typ_subst_fresh S T) in H3; auto with sets.
-      disjoint_solve.
-    auto with sets.
-  destruct (S.union_1 H1); clear Hx H1.
-    use (typ_fv_decr _ _ _ H H0 H2).
-    apply* remove_subset.
-    intros y Hy.
-    destruct (S.union_1 Hy).
-      rewrite <- (@typ_subst_fresh S T) in H3; auto with sets.
-      disjoint_solve.
-    auto with sets.
-  use (IHpairs H H0 _ H2).
-  apply* remove_subset.
-  simpl.
-  rewrite* get_notin_dom.
-  intros y Hy.
-  clear H1 H2.
-  simpl in Hy.
-  destruct (S.union_1 Hy). auto with sets.
-  destruct (S.union_1 H1); auto with sets.
-Qed.
-
 Lemma cardinal_decr : forall v T S pairs,
   v # S -> disjoint (typ_fv T) ({{v}} \u dom S) ->
-  S.cardinal (all_fv (add_binding v T S) pairs) <
+  S.cardinal (all_fv (compose (v ~ T) S) pairs) <
   S.cardinal (all_fv S ((typ_fvar v, T) :: pairs)).
 Proof.
   intros.
@@ -685,7 +1592,7 @@ Qed.
 
 Lemma typ_subst_decr : forall v T S T1,
   v # S ->
-  typ_size (typ_subst (add_binding v T S) T1) <=
+  typ_size (typ_subst (compose (v ~ T) S) T1) <=
   typ_size T * typ_size (typ_subst S T1).
 Proof.
   intros.
@@ -705,7 +1612,7 @@ Qed.
 
 Lemma typ_subst_decr_all : forall v T S pairs,
   v # S ->
-  all_size (add_binding v T S) pairs <= typ_size T * all_size S pairs.
+  all_size (compose (v ~ T) S) pairs <= typ_size T * all_size S pairs.
 Proof.
   unfold all_size; induction pairs; intros; simpl. omega.
   repeat rewrite mult_plus_distr_l.
@@ -717,12 +1624,12 @@ Qed.
 
 Lemma size_pairs_decr : forall v T S pairs,
   v # S -> disjoint (typ_fv T) ({{v}} \u dom S) ->
-  size_pairs (add_binding v T S) pairs < size_pairs S ((typ_fvar v,T)::pairs).
+  size_pairs (compose (v ~ T) S) pairs < size_pairs S ((typ_fvar v,T)::pairs).
 Proof.
   intros.
   unfold size_pairs.
   use (cardinal_decr T S pairs H H0).
-  set (S.cardinal (all_fv (add_binding v T S) pairs)) in *.
+  set (S.cardinal (all_fv (compose (v ~ T) S) pairs)) in *.
   set (S.cardinal (all_fv S ((typ_fvar v, T) :: pairs))) in *.
   clearbody n n0.
   destruct n0; try omega.
@@ -789,8 +1696,8 @@ Lemma typ_subst_eq_add : forall S S0 v T T1 T2 pairs,
   v # S0 ->
   typ_subst S (typ_fvar v) = typ_subst S T ->
   In (T1, T2) pairs -> 
-  typ_subst S (typ_subst (add_binding v T S0) T1) =
-  typ_subst S (typ_subst (add_binding v T S0) T2).
+  typ_subst S (typ_subst (compose (v ~ T) S0) T1) =
+  typ_subst S (typ_subst (compose (v ~ T) S0) T2).
 Proof.
   intros.
   repeat rewrite* typ_subst_add_binding.
@@ -843,7 +1750,7 @@ Lemma unify_complete_step : forall pairs S0 S v T h t t0,
     typ_subst S (typ_subst S0 T1) = typ_subst S (typ_subst S0 T2)) ->
   T <> typ_fvar v ->
   S.mem v (typ_fv T) = false /\
-  exists S', unify pairs (add_binding v T S0) h = Some S'.
+  exists S', unify pairs (compose (v ~ T) S0) h = Some S'.
 Proof.
   intros until t0; intros R1 R2 Hsz HS0 IHh Heq HT.
   case_eq (S.mem v (typ_fv T)); intros.
@@ -864,7 +1771,7 @@ Proof.
   use (size_pairs_decr' _ _ _ HS0 H Hsz R1).
   rewrite R2 in H0; simpl in H0.
   use (typ_subst_res_fresh _ HS0 R1).
-  destruct* (IHh (add_binding v T S0)); clear IHh.
+  destruct* (IHh (compose (v ~ T) S0)); clear IHh.
     apply* add_binding_is_subst.
     use (typ_subst_disjoint t0 HS0).
     rewrite R2 in *; simpl in *.
